\documentclass[11pt, oneside]{article}   	% use "amsart" instead of "article" for AMSLaTeX format
\usepackage{geometry}                		% See geometry.pdf to learn the layout options. There are lots.
\geometry{letterpaper}                   		% ... or a4paper or a5paper or ... 
%\geometry{landscape}                		% Activate for rotated page geometry
%\usepackage[parfill]{parskip}    		% Activate to begin paragraphs with an empty line rather than an indent
\usepackage{graphicx}				% Use pdf, png, jpg, or epsÂ§ with pdflatex; use eps in DVI mode
								% TeX will automatically convert eps --> pdf in pdflatex		
\usepackage{amssymb}

%SetFonts

%SetFonts


\title{Algebra Scratch Work for Assignment 6}
\author{Michael}
%\date{}							% Activate to display a given date or no date

\begin{document}
\maketitle

\section{}
$ p_t = E_t m_{t+1} E_t (c_{t+1} + p_{t+1}) + cov_t (m_{t+1}, c_{t+1} + p_{t+1})$

Recall $c_{t+1} = \lambda_{t+1} c_t$ and $p_t = v_t c_t$

$v_t c_t = E_t[m_{t+1}] E_t[c_{t+1} + p_{t+1}] + E_t[m_{t+1} \times (c_{t+1} + p_{t+1})] - E_t[m_{t+1}] E_t[c_{t+1} + p_{t+1}]$

$v_t c_t = E_t[m_{t+1}] E_t[\lambda_{t+1} c_{t} + v_{t+1} \lambda_{t+1} c_t] + E_t[m_{t+1} \times (\lambda_{t+1} c_{t} + v_{t+1} \lambda_{t+1} c_t)] - E_t[m_{t+1}] E_t[\lambda_{t+1} c_{t} + v_{t+1} \lambda_{t+1} c_t]$

Cancelling out all of the $c_t$ terms we get:

$v_t = E_t[m_{t+1}] E_t[\lambda_{t+1} + v_{t+1} \lambda_{t+1}] + E_t[m_{t+1} \times (\lambda_{t+1} + v_{t+1} \lambda_{t+1})] - E_t[m_{t+1}] E_t[\lambda_{t+1} + v_{t+1} \lambda_{t+1}]$

Simplifying a bit further we get:

$v_t = E_t[m_{t+1} \times (\lambda_{t+1} + v_{t+1} \lambda_{t+1})]$

Now to put this in a form where we can verify the given data in Python:

$v_i = \Sigma_{j=1}^n P_{ij} m_j (s_j + s_j v_j)$

Let $\hat{P}_{ij} = P_{ij}m_j$ 

Then: $v=\hat{P}s + \hat{P} s v$

\section{}
$1 = E_t m_{t+1} E_t R_{t+1} + cov_t (m_{t+1} R_{t+1})$
$1 = E_t m_{t+1} E_t R_{t+1} + E_t (m_{t+1} R_{t+1}) - E_t m_{t+1} E_t R_{t+1}$
$1 = E_t (m_{t+1} R_{t+1})$

\section{}
$v_i = \Sigma_{j=1}^n P_{ij} m_j (s_j + s_j v_j)$

$v = Pms + Pmsv$

$v - Pmsv = Pms$

$v (I-Pms) = Pms$

\end{document}  